core/TraceLink.v
@@ -18,32 +18,61 @@ Context {tc: TransformationConfiguration}.
         We introduce the concept of trace in the syntax to track relationship of a target element and 
         the source pattern that generates it   *)
 
-Inductive TraceLink : Type :=
-  buildTraceLink : 
-    (list SourceElementType * nat * string)
-    -> TargetElementType
-    -> TraceLink.
+Record TraceLink : Type :=
+  buildTraceLink  
+    { 
+      source : (list SourceElementType) * nat * string ;
+      target : TargetElementType 
+    }.
 
 Definition TraceLink_getSourcePattern (tl: TraceLink):=
-  match tl with 
-    buildTraceLink (sp, i, n) te => sp
+  match tl.(source) with 
+    (sp, i, n)  => sp
   end.
 
 Definition TraceLink_getIterator (tl: TraceLink):=
-  match tl with 
-    buildTraceLink (sp, i, n) te => i
+  match tl.(source) with 
+    (sp, i, n)  => i
   end.
 
 Definition TraceLink_getName (tl: TraceLink):=
-  match tl with 
-    buildTraceLink (sp, i, n) te => n
+  match tl.(source) with 
+     (sp, i, n) => n
   end.
 
-Definition TraceLink_getTargetElement (tl: TraceLink):=
-  match tl with 
-    buildTraceLink (sp, i, n) te => te
+Open Scope bool_scope.
+
+
+Definition source_compare (s:(list SourceElementType) * nat * string) (t:TraceLink) : bool :=
+  match s with 
+    (e,i,n) =>
+      list_beq tc.(SourceElement_eqb) (TraceLink_getSourcePattern t) e
+      && Nat.eqb (TraceLink_getIterator t) i
+      && String.eqb (TraceLink_getName t) n
   end.
+
+
+
+Lemma source_compare_refl : 
+  (forall a,  SourceElement_eqb a a = true) ->
+  forall a b, 
+    source_compare a {| source := a ; target := b |} = true.
+Proof.
+  intro R.    
+  intros a b.
+  destruct a. destruct p.
+  unfold source_compare.
+  unfold TraceLink_getSourcePattern ; simpl.
+  unfold TraceLink_getIterator ; simpl.
+  unfold TraceLink_getName ; simpl.
+  rewrite list_beq_refl ; [ | exact R].
+  rewrite NPeano.Nat.eqb_refl.
+  rewrite String.eqb_refl. 
+  reflexivity.
+Qed.
 
 End TraceLink.
 
 Arguments TraceLink {_}.
+
+Arguments source_compare : simpl never.
